Tests/Issues.lean
@@ -1,15 +1,15 @@
 
 import Tests.Issues.Issue1
--- import Tests.Issues.Issue2
--- import Tests.Issues.Issue3
--- import Tests.Issues.Issue4
--- import Tests.Issues.Issue5
+import Tests.Issues.Issue2
+import Tests.Issues.Issue3
+import Tests.Issues.Issue4
+import Tests.Issues.Issue5
 import Tests.Issues.Issue6
 import Tests.Issues.Issue7
 import Tests.Issues.Issue8
 import Tests.Issues.Issue9
 import Tests.Issues.Issue10
--- import Tests.Issues.Issue11
+import Tests.Issues.Issue11
 import Tests.Issues.Issue12
 import Tests.Issues.Issue14
 import Tests.Issues.Issue15
@@ -18,3 +18,10 @@ import Tests.Issues.Issue17
 import Tests.Issues.Issue18
 import Tests.Issues.Issue19
 import Tests.Issues.Issue20
+import Tests.Issues.Issue21
+import Tests.Issues.Issue22
+import Tests.Issues.Issue23
+import Tests.Issues.Issue24
+import Tests.Issues.Issue25
+import Tests.Issues.Issue26
+import Tests.Issues.Issue27
