Tests/Issues/Issue24.lean
@@ -1,0 +1,35 @@
+import Lean
+import Solver.Command.Tactic
+
+open Lean Meta
+namespace Tests.Issue24
+
+-- Issue: translateApp: unexpected application Lean.Expr.app (Lean.Expr.const `Tests.Issue24.blake256 []) ...
+-- Diagnosis : We need to consider not prop axiom during smt translation to properly
+--             generate global variables.
+
+
+axiom hash : String → String
+axiom hash_collision_prop1 : ∀ (s1 s2 : String), hash s1 = hash s2 → s1 = s2
+axiom hash_collision_prop2 : ∀ (s1 s2 : String), s1 = s2 → hash s1 = hash s2
+axiom hash_size : ∀ (s : String), (hash s).length = 256
+
+-- check if we have a counterexample of length 256
+-- Remove solver options once performance issue resolved
+#solve (timeout: 5) (solve-result: 2) [∀ (s : String), (hash s).length < 256]
+
+-- validate axiom
+#solve (only-optimize: 1) [∀ (s : String), (hash s).length = 256]
+
+-- check if we are not wrongly applying axiom on another function
+axiom hash2 : String → String
+-- Remove solver options once performance issue resolved
+#solve (timeout: 5) (solve-result: 2) [∀ (s : String), (hash2 s).length = 256]
+#solve (timeout: 5) (solve-result: 2) [∀ (s : String) (f : String → String), (f s).length = 256]
+
+-- check when axiom function is passed as argument
+#solve (random-seed: 1)
+       [ ∀ (xs : List String), !(List.isEmpty xs) → (List.head! (List.map hash xs)).length = 256 ]
+
+
+end Tests.Issue24
